categorical-semantics/Spitters2011/Spitters2011.v
@@ -1,0 +1,74 @@
+(* Spitters & van der Weegen 2011, "Type Classes for Mathematics in Type Theory" *)
+(* https://arxiv.org/pdf/1102.1323.pdf *)
+
+Global Generalizable All Variables.
+
+Set Warnings "-notation-overridden,-parsing,-deprecated-hint-without-locality".
+From Coq Require Import Strings.String.
+
+From Coq.Strings Require Export String.
+From Coq.Lists Require Export List.
+From Coq.Arith Require Export Peano_dec.
+
+From Coq.Relations Require Export Relations.
+From Coq.Classes Require Export Equivalence.
+From Coq.Classes Require Export Morphisms.
+
+(* ====================================================== *)
+
+Class Equiv A := equiv: relation A.
+
+Infix "=" := equiv: type_scope.
+
+Class Associative `{Equiv A} (f : A -> A -> A) := {
+  associativity : forall x y z, f x (f y z) = f (f x y) z
+}.
+
+(* ====================================================== *)
+Module SemiGroup_Record.
+
+Record SemiGroup (G : Type) (H: Equiv G) (e : relation G) (op : G -> G -> G) : Prop :=
+  { sg_setoid : Equivalence e
+  ; sg_assoc  : Associative op
+  ; sg_proper : Proper (e ==> e ==> e) op }.
+
+End SemiGroup_Record.
+(* ====================================================== *)
+(* ====================================================== *)
+Module SemiGroup_TypeClass.
+
+Class SemiGroup (G : Type) `{Equiv G} (e : relation G) (op : G -> G -> G) : Prop :=
+  { sg_setoid : Equivalence e
+  ; sg_assoc  : Associative op
+  ; sg_proper : Proper (e ==> e ==> e) op }.
+
+(* example theorem, "vanilla" approach *)
+Theorem example_theorem `{SemiGroup G e op}:
+  forall x y z,
+    e (op (op x y) z) (op (op z y) x).
+Admitted.
+
+End SemiGroup_TypeClass.
+(* ====================================================== *)
+(* ====================================================== *)
+Module SemiGroup_OperationalTypeClass.
+
+(* an "operational type class" *)
+Class SemiGroupOp A := sg_op : A -> A -> A.
+Infix "&" := sg_op (at level 50, left associativity).
+
+Record SemiGroup (G : Type) (eq : Equiv G) (op : SemiGroupOp G) : Prop :=
+  { sg_setoid : Equivalence equiv
+  ; sg_assoc  : Associative op
+  ; sg_proper : Proper (equiv ==> equiv ==> equiv) op }.
+
+(* example theorem, "operational type class" approach *)
+Theorem example01 G eq op `{SemiGroup G eq op}:
+  forall x y z,
+    x & y & z = z & y & x.
+Admitted.
+
+End SemiGroup_OperationalTypeClass.
+(* ====================================================== *)
+(* ====================================================== *)
+
